src/program_logic/crash_inv.v
@@ -19,54 +19,57 @@ Implicit Types Φc : iProp Σ.
 Implicit Types v : val Λ.
 Implicit Types e : expr Λ.
 
-Definition crash_inv N k E γ P :=
-  (∃ γ', staged_inv N k (E ∖ ↑N) (E ∖ ↑N) γ γ' P)%I.
+Definition crash_inv N k E P :=
+  (∃ γ γ', staged_inv N k (E ∖ ↑N) (E ∖ ↑N) γ γ' P)%I.
 
-Definition crash_inv_full N k E γ Q P :=
-  (∃ γ' Qr, staged_inv N k (E ∖ ↑N) (E ∖ ↑N) γ γ' P ∗ staged_value N γ Q Qr ∗ □ (Q -∗ P))%I.
+Definition crash_inv_full N k E Q P :=
+  (∃ γ γ' Qr, staged_inv N k (E ∖ ↑N) (E ∖ ↑N) γ γ' P ∗ staged_value N γ Q Qr ∗ □ (Q -∗ P))%I.
 
-Definition crash_inv_pending N k E γ P :=
-  (∃ γ', staged_inv N k (E ∖ ↑N) (E ∖ ↑N) γ γ' P ∗ staged_pending γ')%I.
+Definition crash_inv_pending N k E P :=
+  (∃ γ γ', staged_inv N k (E ∖ ↑N) (E ∖ ↑N) γ γ' P ∗ staged_pending γ')%I.
 
-Global Instance crash_inv_pers N k E γ P : Persistent (crash_inv N k E γ P).
+Global Instance crash_inv_pers N k E P : Persistent (crash_inv N k E P).
 Proof. apply _. Qed.
 
 Lemma crash_inv_alloc N k E E' P Q:
   ▷ Q ∗ □ (Q -∗ P) ={E}=∗
-  ∃ γ, crash_inv_full N k E' γ Q P ∗ crash_inv_pending N k E' γ P.
+  crash_inv_full N k E' Q P ∗ crash_inv_pending N k E' P.
 Proof.
   iIntros "HQP".
   iDestruct "HQP" as "(HQ&#HQP)".
   iMod (staged_inv_alloc N k E (E' ∖ ↑N) P Q True%I with "[HQ]") as (γ γ') "(#Hinv&Hval&Hpend)".
   { iFrame. iAlways. iIntros. iDestruct ("HQP" with "[$]") as "$". }
   iModIntro.
-  iExists γ.
   iSplitL "Hval".
-  - iExists γ', _. iFrame. iFrame "Hinv". iAlways; eauto.
-  - iExists _. iFrame. iFrame "Hinv".
+  - iExists γ, γ', _. iFrame. iFrame "Hinv". iAlways; eauto.
+  - iExists γ, _. iFrame. iFrame "Hinv".
 Qed.
 
-Lemma crash_inv_full_weaken N k E γ Q P:
-  crash_inv_full N k E γ Q P -∗ crash_inv N k E γ P.
-Proof. iIntros "H". iDestruct "H" as (??) "(?&?)"; eauto. iExists _. iFrame. Qed.
+Lemma crash_inv_full_impl N k E Q P:
+  crash_inv_full N k E Q P -∗ □ (Q -∗ P).
+Proof. iIntros "H". iDestruct "H" as (???) "(?&?&$)"; eauto. Qed.
 
-Lemma crash_inv_pending_weaken N k E γ P:
-  crash_inv_pending N k E γ P -∗ crash_inv N k E γ P.
-Proof. iIntros "H". iDestruct "H" as (?) "(?&?)"; eauto. iExists _. iFrame. Qed.
+Lemma crash_inv_full_weaken N k E Q P:
+  crash_inv_full N k E Q P -∗ crash_inv N k E P.
+Proof. iIntros "H". iDestruct "H" as (???) "(?&?)"; eauto. iExists _, _. iFrame. Qed.
 
-Lemma wpc_crash_inv_open s k k' E1 E1' E2 e Φ Φc Q P N γ :
+Lemma crash_inv_pending_weaken N k E P:
+  crash_inv_pending N k E P -∗ crash_inv N k E P.
+Proof. iIntros "H". iDestruct "H" as (??) "(?&?)"; eauto. iExists _, _. iFrame. Qed.
+
+Lemma wpc_crash_inv_open s k k' E1 E1' E2 e Φ Φc Q P N:
   E1 ⊆ E1' →
   ↑N ⊆ E1 →
   S k < k' →
   to_val e = None →
-  crash_inv_full N (LVL k') E1' γ Q P -∗
+  crash_inv_full N (LVL k') E1' Q P -∗
   (Φc ∧ (Q -∗ WPC e @ NotStuck; (LVL k); (E1 ∖ ↑N); ∅
-                    {{λ v, Q ∗ (crash_inv_full N (LVL k') E1' γ Q P -∗ (Φ v ∧ Φc))}}
+                    {{λ v, Q ∗ (crash_inv_full N (LVL k') E1' Q P -∗ (Φ v ∧ Φc))}}
                     {{ Φc ∗ P }})) -∗
   WPC e @ s; LVL (S (S k)); E1; E2 {{ Φ }} {{ Φc }}.
 Proof.
   iIntros (????) "Hfull Hwp".
-  iDestruct "Hfull" as (??) "(#Hinv&Hval&#Hwand)".
+  iDestruct "Hfull" as (???) "(#Hinv&Hval&#Hwand)".
   iApply (wpc_staged_inv_open _ _ _ _ _ _ _ _ _ _ _ (λ _, Q)); eauto.
   iFrame "Hinv". iFrame.
   iSplit.
@@ -78,23 +81,23 @@ Proof.
   - iIntros (?) "(HQ&HQrest)".
     iModIntro. iFrame "HQ".
     iFrame "Hwand". iIntros.
-    iApply "HQrest". iExists _, _. iFrame. iFrame "Hinv". iFrame "Hwand".
+    iApply "HQrest". iExists _, _, _. iFrame. iFrame "Hinv". iFrame "Hwand".
   - iIntros. rewrite difference_diag_L. iModIntro; eauto.
 Qed.
 
-Lemma wpc_crash_inv_open_modify Qnew s k k' E1 E1' E2 e Φ Φc Q P N γ :
+Lemma wpc_crash_inv_open_modify Qnew s k k' E1 E1' E2 e Φ Φc Q P N :
   E1 ⊆ E1' →
   ↑N ⊆ E1 →
   S k < k' →
   to_val e = None →
-  crash_inv_full N (LVL k') E1' γ Q P -∗
+  crash_inv_full N (LVL k') E1' Q P -∗
   (Φc ∧ (Q -∗ WPC e @ NotStuck; (LVL k); (E1 ∖ ↑N); ∅
-                    {{λ v, Qnew v ∗ □ (Qnew v -∗ P)  ∗ (crash_inv_full N (LVL k') E1' γ (Qnew v) P -∗ (Φ v ∧ Φc))}}
+                    {{λ v, Qnew v ∗ □ (Qnew v -∗ P)  ∗ (crash_inv_full N (LVL k') E1' (Qnew v) P -∗ (Φ v ∧ Φc))}}
                     {{ Φc ∗ P }})) -∗
   WPC e @ s; LVL (S (S k)); E1; E2 {{ Φ }} {{ Φc }}.
 Proof.
   iIntros (????) "Hfull Hwp".
-  iDestruct "Hfull" as (??) "(#Hinv&Hval&#Hwand)".
+  iDestruct "Hfull" as (???) "(#Hinv&Hval&#Hwand)".
   iApply (wpc_staged_inv_open _ _ _ _ _ _ _ _ _ _ _ Qnew); eauto.
   iFrame "Hinv". iFrame.
   iSplit.
@@ -105,56 +108,31 @@ Proof.
   iSplit.
   - iIntros (?) "(HQ&#Hwand'&HQrest)".
     iModIntro. iFrame "HQ Hwand'". iIntros "Hval".
-    iApply "HQrest". iExists _, _. iFrame. iFrame "Hinv". iFrame "Hwand'".
+    iApply "HQrest". iExists _, _, _. iFrame. iFrame "Hinv". iFrame "Hwand'".
   - iIntros. rewrite difference_diag_L. iModIntro; eauto.
 Qed.
 
-Lemma wpc_crash_inv_init s k k' N E1 E2 e Φ Φc P γ :
+Lemma wpc_crash_inv_init s k k' N E1 E2 e Φ Φc P :
   k' < k →
   ↑N ⊆ E1 →
-  crash_inv_pending N (LVL k') E1 γ P ∗
+  crash_inv_pending N (LVL k') E1 P ∗
   WPC e @ s; LVL k; E1; E2 {{ Φ }} {{ Φc }} ⊢
   WPC e @ s; LVL (S k); E1; E2 {{ Φ }} {{ Φc ∗ P }}.
 Proof.
   iIntros (??) "(H&?)".
-  iDestruct "H" as (?) "(?&?)".
+  iDestruct "H" as (??) "(?&?)".
   iApply wpc_staged_inv_init; last (by iFrame); eauto.
 Qed.
 
-Lemma crash_inv_open N k' k E E' E1 γ P Q R:
+Lemma crash_inv_open_modify N k' k E E' E1 P Q R:
   ↑N ⊆ E →
-  crash_inv_full N k' E1 γ Q P -∗
-  ((Q ∗ (▷ Q ={E∖↑N,E}=∗ crash_inv_full N k' E1 γ Q P)) ∨ (C ∗ |={E∖↑N, E}=> crash_inv_full N k' E1 γ Q P)
+  crash_inv_full N k' E1 Q P -∗
+  ((Q ∗ (∀ Q', ▷ Q' ∗ □ (Q' -∗ P) ={E∖↑N,E}=∗ crash_inv_full N k' E1 Q' P)) ∨ (C ∗ |={E∖↑N, E}=> crash_inv_full N k' E1 Q P)
    -∗ |={E ∖ ↑N, E'}_k=> R) -∗
   (|={E,E'}_(S (S k))=> R).
 Proof.
   iIntros (?) "H Hwp".
-  iDestruct "H" as (??) "(#Hinv&H&#Hwand)".
-  iMod (staged_inv_open with "[H]") as "HQ"; try iFrame "H Hinv"; eauto.
-  iMod (fupd_intro_mask' _ ∅) as "Hclo"; first set_solver.
-  iModIntro.
-  rewrite Nat_iter_S.
-  iModIntro. iNext. iModIntro.
-  rewrite Nat_iter_S.
-  iModIntro. iNext. iMod "Hclo" as "_".
-  iApply ("Hwp" with "[HQ]").
-  iDestruct "HQ" as "[(HQ&Hclo)|(?&HC&Hclo)]".
-  - iLeft. iFrame. iIntros "HQ". iMod ("Hclo" $! Q True%I with "[HQ]") as "H".
-    { iFrame. iAlways. iIntros. iApply step_fupdN_inner_later; auto. iNext.
-      iDestruct ("Hwand" with "[$]") as "$". }
-    iModIntro. iExists _, _. iFrame "H Hinv Hwand".
-  - iRight. iFrame. iMod "Hclo". iModIntro. iExists _, _. iFrame "Hclo Hwand Hinv".
-Qed.
-
-Lemma crash_inv_open_modify N k' k E E' E1 γ P Q R:
-  ↑N ⊆ E →
-  crash_inv_full N k' E1 γ Q P -∗
-  ((Q ∗ (∀ Q', ▷ Q' ∗ □ (Q' -∗ P) ={E∖↑N,E}=∗ crash_inv_full N k' E1 γ Q' P)) ∨ (C ∗ |={E∖↑N, E}=> crash_inv_full N k' E1 γ Q P)
-   -∗ |={E ∖ ↑N, E'}_k=> R) -∗
-  (|={E,E'}_(S (S k))=> R).
-Proof.
-  iIntros (?) "H Hwp".
-  iDestruct "H" as (??) "(#Hinv&H&#Hwand)".
+  iDestruct "H" as (???) "(#Hinv&H&#Hwand)".
   iMod (staged_inv_open with "[H]") as "HQ"; try iFrame "H Hinv"; eauto.
   iMod (fupd_intro_mask' _ ∅) as "Hclo"; first set_solver.
   iModIntro.
@@ -167,8 +145,23 @@ Proof.
   - iLeft. iFrame. iIntros (Q') "(HQ'&#Hwand')". iMod ("Hclo" $! Q' True%I with "[HQ']") as "H".
     { iFrame. iAlways. iIntros. iApply step_fupdN_inner_later; auto. iNext.
       iDestruct ("Hwand'" with "[$]") as "$". }
-    iModIntro. iExists _, _. iFrame "H Hinv Hwand'".
-  - iRight. iFrame. iMod "Hclo". iModIntro. iExists _, _. iFrame "Hclo Hwand Hinv".
+    iModIntro. iExists _, _, _. iFrame "H Hinv Hwand'".
+  - iRight. iFrame. iMod "Hclo". iModIntro. iExists _, _, _. iFrame "Hclo Hwand Hinv".
+Qed.
+
+Lemma crash_inv_open N k' k E E' E1 P Q R:
+  ↑N ⊆ E →
+  crash_inv_full N k' E1 Q P -∗
+  ((Q ∗ (▷ Q ={E∖↑N,E}=∗ crash_inv_full N k' E1 Q P)) ∨ (C ∗ |={E∖↑N, E}=> crash_inv_full N k' E1 Q P)
+   -∗ |={E ∖ ↑N, E'}_k=> R) -∗
+  (|={E,E'}_(S (S k))=> R).
+Proof.
+  iIntros (?) "H1 H2". iDestruct (crash_inv_full_impl with "[$]") as "#HQP".
+  iApply (crash_inv_open_modify with "[$]"); first done.
+  iIntros "Hwand". iApply ("H2" with "[Hwand]").
+  iDestruct "Hwand" as "[H1|H2]".
+   - iLeft. iDestruct "H1" as "($&H)". iIntros "HQ". by iMod ("H" $! Q with "[$]").
+   - iRight. iFrame.
 Qed.
 
 End ci.
